Porting CompCert-CertiKOS to CompCert 2.7.1
In particular Stackingproof has been changed a lot (use of separation logic)

cfrontend/Cexec.v
@@ -730,6 +730,16 @@ Notation " 'check' A ; B" := (if A then B else stuck)
 
 Local Open Scope reducts_monad_scope.
 
+Definition builtin_is_enabled (ef: external_function) :
+  {builtin_enabled ef} + {~ builtin_enabled ef}.
+Proof.
+  unfold builtin_enabled.
+  destruct ef; try (left; exact I).
+  destruct cc_enable_external_as_builtin.
+  left. exact I.
+  right; intro; assumption.
+Defined.
+
 Fixpoint step_expr (k: kind) (a: expr) (m: mem): reducts expr :=
   match k, a with
   | LV, Eloc b ofs ty =>
@@ -915,11 +925,13 @@ Fixpoint step_expr (k: kind) (a: expr) (m: mem): reducts expr :=
   | RV, Ebuiltin ef tyargs rargs ty =>
       match is_val_list rargs with
       | Some vtl =>
-          do vargs <- sem_cast_arguments vtl tyargs m;
-          match do_external ef w vargs m with
-          | None => stuck
-          | Some(w',t,v,m') => topred (Rred "red_builtin" (Eval v ty) m' t)
-          end
+        do vargs <- sem_cast_arguments vtl tyargs m;
+          if builtin_is_enabled ef then
+            match do_external ef w vargs m with
+            | None => stuck
+            | Some(w',t,v,m') => topred (Rred "red_builtin" (Eval v ty) m' t)
+            end
+          else stuck
       | _ =>
           incontext (fun x => Ebuiltin ef tyargs x ty) (step_exprlist rargs m)
       end
@@ -1025,9 +1037,10 @@ Definition invert_expr_prop (a: expr) (m: mem) : Prop :=
       /\ cast_arguments m rargs tyargs vl
       /\ type_of_fundef fd = Tfunction tyargs tyres cconv
   | Ebuiltin ef tyargs rargs ty =>
-      exprlist_all_values rargs ->
-      exists vargs t vres m' w',
-         cast_arguments m rargs tyargs vargs
+    exprlist_all_values rargs ->
+    builtin_enabled ef /\
+    exists vargs t vres m' w',
+      cast_arguments m rargs tyargs vargs
       /\ external_call ef ge vargs m t vres m'
       /\ possible_trace w t w'
   | _ => True
@@ -1059,7 +1072,7 @@ Proof.
   exists t; exists v1; exists w'; auto.
   exists t; exists v1; exists w'; auto.
   exists v; auto.
-  intros; exists vargs; exists t; exists vres; exists m'; exists w'; auto.
+  intros; split. apply BUILTIN_ENABLED. exists vargs; exists t; exists vres; exists m'; exists w'; auto.
 Qed.
 
 Lemma callred_invert:
@@ -1533,9 +1546,11 @@ Proof with (try (apply not_invert_ok; simpl; intro; myinv; intuition congruence;
   destruct (sem_cast_arguments vtl tyargs m) as [vargs|] eqn:?...
   destruct (do_external ef w vargs m) as [[[[? ?] v] m'] | ] eqn:?...
   exploit do_ef_external_sound; eauto. intros [EC PT].
+  destruct (builtin_is_enabled ef) eqn:?...
   apply topred_ok; auto. red. split; auto. eapply red_builtin; eauto.
   eapply sem_cast_arguments_sound; eauto.
   exists w0; auto.
+  destruct (builtin_is_enabled ef) eqn:?...
   apply not_invert_ok; simpl; intros; myinv. specialize (H ALLVAL). myinv.
   assert (x = vargs).
     exploit sem_cast_arguments_complete; eauto. intros [vtl' [A B]]. congruence.
@@ -1637,6 +1652,7 @@ Proof.
   inv H0. rewrite H; econstructor; eauto.
 (* builtin *)
   exploit sem_cast_arguments_complete; eauto. intros [vtl [A B]].
+  destruct (builtin_is_enabled ef); try contradiction.
   exploit do_ef_external_complete; eauto. intros C.
   rewrite A. rewrite B. rewrite C. econstructor; eauto.
 Qed.
