backend/CSEproof.v
@@ -110,7 +110,7 @@ Ltac splitall := repeat (match goal with |- _ /\ _ => split end).
 
 Section WITHEXTERNALCALLS.
 Context `{external_calls_prf: ExternalCalls}.
-
+ 
 Lemma valnum_reg_holds:
   forall valu1 ge sp rs m n r n' v,
   numbering_holds valu1 ge sp rs m n ->
