backend/CleanupLabelsproof.v
@@ -289,7 +289,7 @@ Proof.
   econstructor.
   eapply eval_builtin_args_preserved with (ge1 := ge); eauto. exact symbols_preserved.
   eapply external_call_symbols_preserved; eauto. apply senv_preserved.
-  eauto.
+  eauto. auto.
   econstructor; eauto with coqlib.
 (* Llabel *)
   case_eq (Labelset.mem lbl (labels_branched_to (fn_code f))); intros.
