backend/Cminor.v
@@ -482,6 +482,7 @@ Inductive step: state -> trace -> state -> Prop :=
   | step_builtin: forall f optid ef bl k sp e m vargs t vres m',
       eval_exprlist sp e m bl vargs ->
       external_call ef ge vargs m t vres m' ->
+      forall BUILTIN_ENABLED : builtin_enabled ef,
       step (State f (Sbuiltin optid ef bl) k sp e m)
          t (State f Sskip k sp (set_optvar optid vres e) m')
 
@@ -700,6 +701,7 @@ with exec_stmt:
       eval_exprlist ge sp e m bl vargs ->
       external_call ef ge vargs m t vres m' ->
       e' = set_optvar optid vres e ->
+      forall BUILTIN_ENABLED : builtin_enabled ef,
       exec_stmt f sp e m (Sbuiltin optid ef bl) t e' m' Out_normal
   | exec_Sifthenelse:
       forall f sp e m a s1 s2 v b t e' m' out,
