backend/SelectDivproof.v
@@ -329,7 +329,7 @@ Qed.
 (** * Correctness of the smart constructors for division and modulus *)
 
 Section CMCONSTRS.
-Context `{external_calls_ops: ExternalCallsOps}.
+Context `{external_calls: ExternalCalls}.
 
 Variable ge: genv.
 Variable sp: val.
