cfrontend/Csharpminor.v
@@ -262,7 +262,7 @@ Definition eval_constant (cst: constant) : option val :=
 Definition eval_unop := Cminor.eval_unop.
 
 Section WITHEXTERNALCALLSOPS.
-Context `{external_calls_ops: ExternalCallsOps}.
+Context `{external_calls_prf: ExternalCalls}.
 
 Definition eval_binop := Cminor.eval_binop.
 
@@ -396,6 +396,7 @@ Inductive step: state -> trace -> state -> Prop :=
   | step_builtin: forall f optid ef bl k e le m vargs t vres m',
       eval_exprlist e le m bl vargs ->
       external_call ef ge vargs m t vres m' ->
+      forall BUILTIN_ENABLED: builtin_enabled ef,
       step (State f (Sbuiltin optid ef bl) k e le m)
          t (State f Sskip k e (Cminor.set_optvar optid vres le) m')
 
