ia32/Stacklayout.v
@@ -99,6 +99,38 @@ Local Opaque Z.add Z.mul sepconj range.
   exact H.
 Qed.
 
+Lemma frame_env_separated':
+  forall `{memory_model_prf: Mem.MemoryModel},
+  forall b ,
+    let fe := make_env b in
+     let olink := 4 * bound_outgoing b in
+     let ocs := olink + 4 in
+     let ol := align (size_callee_save_area b ocs) 8 in
+     let ostkdata := align (ol + 4 * bound_local b) 8 in
+     let oretaddr := align (ostkdata + bound_stack_data b) 4 in
+     0 <= olink
+  /\ olink + 4 <= ocs
+  /\ ocs <= size_callee_save_area b ocs
+  /\ size_callee_save_area b ocs <= ol
+  /\ ol + 4 * bound_local b <= ostkdata
+  /\ ostkdata + bound_stack_data b <= oretaddr
+  /\ olink <= fe_stack_data fe.
+Proof.
+Local Opaque Z.add Z.mul sepconj range fe_stack_data.
+  intros; simpl.
+  generalize b.(bound_local_pos) b.(bound_outgoing_pos) b.(bound_stack_data_pos); intros.
+  assert (0 <= olink) by (unfold olink; omega).
+  assert (olink + 4 <= ocs) by (unfold ocs; omega).
+  assert (ocs <= size_callee_save_area b ocs) by (apply size_callee_save_area_incr).
+  assert (size_callee_save_area b ocs <= ol) by (apply align_le; omega).
+  assert (ol + 4 * b.(bound_local) <= ostkdata) by (apply align_le; omega).
+  assert (ostkdata + bound_stack_data b <= oretaddr) by (apply align_le; omega).
+  repeat split; auto.
+  Local Transparent fe_stack_data.
+  simpl. fold olink. fold ocs. fold ol. fold ostkdata.
+  omega.
+Qed.
+
 Lemma frame_env_range:
   forall b,
   let fe := make_env b in
